proof/spec/LTree.ec
@@ -1,0 +1,64 @@
+pragma Goals : printall.
+
+
+require import AllCore List RealExp IntDiv Distr DList.
+require (*--*) Subtype. 
+
+from Jasmin require import JModel.
+ 
+require import Params Address Hash WOTS.
+ 
+
+op H : nbytes -> nbytes -> nbytes.
+op H_msg : threen_bytes -> W8.t list -> nbytes.
+
+clone export Subtype as WOTSKeys with 
+   type T = wots_sk list,
+   op P = fun l => size l = 2^h
+   rename "T" as "wots_keys".
+
+(* 4.1.5 L-Trees *)
+(* takes as input a WOTS+ public key pk and compresses it to a single 
+   n-byte value pk[0].
+*)
+module LTree = {
+  proc ltree (pk : wots_pk, address : adrs, _seed : seed) : nbytes * adrs = {
+    var pk_i : nbytes;
+    var tmp : nbytes;
+    var i : int <- witness;
+    var _len : int <- len;
+    var tree_height : int;
+
+    address <- set_tree_height address 0;
+
+    while (1 < _len) { (* Same as _len > 1 *)
+      i <- 0;
+      while (i < _len %/ 2) {
+        address <- set_tree_index address i;
+        pk_i <- nth witness pk (2*i);
+        tmp <- nth witness pk (2*i + 1);
+        (pk_i, address) <@ Hash.rand_hash (pk_i, tmp, _seed, address);
+        pk <- put pk i pk_i;
+        i <- i + 1;
+      }
+
+      if (_len %% 2 = 1) {
+        pk_i <- nth witness pk (_len - 1);
+        pk <- put pk (_len %/ 2) pk_i;
+      }
+
+      _len <- if _len %% 2 = 0 then _len %/ 2 else _len %/ 2 + 1;
+
+      tree_height <- get_tree_height address;
+      address <- set_tree_height address (tree_height + 1);
+    }
+
+    pk_i <- nth witness pk 0;
+
+    return (pk_i, address);
+  }
+}. 
+
+
+lemma ltree_ll : islossless LTree.ltree.
+admitted.
