proof/spec/Params.ec
@@ -1,0 +1,49 @@
+require import AllCore List RealExp IntDiv.
+require Subtype.
+
+from Jasmin require import JModel.
+
+(* Height of the overall Merkle tree *)
+(* XMSS_TREE_HEIGHT in the implementation *)
+const h : { int | 0 < h } as h_g0.
+
+(*  A tree of height h has 2^h leaf nodes *)
+op nr_leaves (h : int) : int = 2^h.
+
+(* Length the digest *)
+const n : { int | 0 <= n } as ge0_n.
+
+(* Winternitz parameter: the range of indices into a wots chain *)
+op w : { int | w = 4 \/ w = 16} as w_vals.
+
+const len1 : int = ceil (8%r * n%r / log2 w%r).
+const len2 : int = floor (log2 (len1 * (w - 1))%r / log2 w%r) + 1.
+const len : int = len1 + len2.
+
+axiom ge0_h : 0 <= h.
+axiom ge0_len  : 0 <= len.
+axiom ge0_len1 : 0 <= len1.
+
+
+clone export Subtype as NBytes with 
+   type T = W8.t list,
+   op P = fun l => size l = n
+   rename "T" as "nbytes".
+
+clone export Subtype as LenNBytes with 
+   type T = nbytes list,
+   op P = fun l => size l = len
+   rename "T" as "len_nbytes".
+
+clone export Subtype as OneByte with 
+   type T = W8.t list,
+   op P = fun l => size l = 1
+   rename "T" as "onebyte".
+
+clone export Subtype as TheeNBytes with 
+   type T = W8.t list,
+   op P = fun l => size l = 3 * n
+   rename "T" as "threen_bytes"
+   proof inhabited by (exists (nseq (3*n) W8.zero);smt(size_nseq ge0_n))
+   proof *.
+
