proof/spec/xmss/XMSS_Types.ec
@@ -1,55 +1,12 @@
 require import AllCore List RealExp IntDiv.
 require (*  *) Subtype. 
 
-require import XMSS_Params.
+require export XMSS_Params WOTS.
 
 from Jasmin require import JModel.
 
 require import Array8.
-
-type adrs = W32.t Array8.t.
-
-type nbytes = W8.t list. (* size = n *)
-type len_n_bytes = nbytes list. (* list of length len, each element of length n *)
-type len1_bytes = W8.t list. (* list of length len1 *)
-
-(******************************************************************************)
-
-type key = nbytes.
-type seed = nbytes.
-
-(******************************************************************************)
-
-type wots_message = nbytes.
-type wots_message_base_w = len1_bytes.
-type wots_signature = len_n_bytes.
-type wots_pk = len_n_bytes.
-type wots_sk = len_n_bytes.
-type wots_keypair = wots_pk * wots_sk.
-
-(******************************************************************************)
-
-clone import Subtype as OTSKeys with 
-   type T = wots_sk list,
-   op P = fun l => size l = 2^h
-   rename "T" as "wots_ots_keys".
-
-clone import Subtype as Three_NBytes with 
-   type T = W8.t list,
-   op P = fun l => size l = 3 * n
-   rename "T" as "three_n_bytes"
-   proof inhabited by (exists (nseq (3*n) W8.zero);smt(size_nseq ge0_n))
-   proof *.
-
-(* treeheight . n *)
-clone import Subtype as AuthPath with
-  type T = nbytes list,
-  op P = fun l => size l = d
-  rename "T" as "auth_path"
-  proof inhabited by admit
-  proof *.
-
-(******************************************************************************)
+import Params.
 
 (* Same as single tree variant *)
 type xmss_sk = { idx : W32.t ;
@@ -64,6 +21,14 @@ type xmss_pk = { pk_oid : W32.t ;
                  pk_pub_seed : nbytes }.
 
 type msg_t = W8.t list.
+
+(* treeheight . n *)
+clone export Subtype as AuthPath with
+  type T = nbytes list,
+  op P = fun l => size l = 1
+  rename "T" as "auth_path"
+  proof inhabited by (exists [witness];auto)
+  proof *.
 
 type reduced_signature = wots_signature * auth_path.
 
