proof/spec/xmss_mt/XMSS_MT_Params.ec
@@ -1,8 +1,8 @@
 require import AllCore List RealExp IntDiv.
 
-(* Height of the overall Merkle tree *)
-(* XMSS_TREE_HEIGHT in the implementation *)
-const h : { int | 0 < h } as h_g0.
+from Jasmin require import JModel.
+
+require export Params.
 
 (* Number of layers in a hypertree in XMSS^MT *)
 (* d = 1 for the single-tree variant *)
@@ -11,24 +11,9 @@ const h : { int | 0 < h } as h_g0.
 (* d layers of trees, each having height h/d  *)
 (* hyper-tree of total height h, where h is a multiple of d *)
 const d : { int | 0 < h /\ h %% d = 0 } as d_g0.
+axiom ge0_d : 0 < d.
 
 (* XMSS_FULL_HEIGHT in the implementation *)
 op full_height (h d : int) : int = h * d.
 
-(*  A tree of height h has 2^h leaf nodes *)
-op nr_leaves (h : int) : int = 2^h.
-
-(* Length the digest *)
-const n : { int | 0 <= n } as ge0_n.
-
-(* Winternitz parameter: the range of indices into a wots chain *)
-op w : { int | w = 4 \/ w = 16} as w_vals.
-
-const len1 : int = ceil (8%r * n%r / log2 w%r).
-const len2 : int = floor (log2 (len1 * (w - 1))%r / log2 w%r) + 1.
-const len : int = len1 + len2.
-
-axiom ge0_h : 0 <= h.
-axiom ge0_len  : 0 <= len.
-axiom ge0_len1 : 0 <= len1.
-axiom ge0_d : 0 < d.
+op impl_oid : W32.t.
