proof/spec/xmss_mt/XMSS_MT_Types.ec
@@ -1,52 +1,19 @@
 require import AllCore List RealExp IntDiv.
 require (*  *) Subtype. 
 
-require import XMSS_Params.
+require import XMSS_MT_Params WOTS.
 
 from Jasmin require import JModel.
 
 require import Array8.
 
-type adrs = W32.t Array8.t.
-
-type nbytes = W8.t list. (* size = n *)
-type len_n_bytes = nbytes list. (* list of length len, each element of length n *)
-type len1_bytes = W8.t list. (* list of length len1 *)
-
-(******************************************************************************)
-
-type key = nbytes.
-type seed = nbytes.
-
-(******************************************************************************)
-
-type wots_message = nbytes.
-type wots_message_base_w = len1_bytes.
-type wots_signature = len_n_bytes.
-type wots_pk = len_n_bytes.
-type wots_sk = len_n_bytes.
-type wots_keypair = wots_pk * wots_sk.
-
-(******************************************************************************)
-
-clone import Subtype as OTSKeys with 
-   type T = wots_sk list,
-   op P = fun l => size l = 2^h
-   rename "T" as "wots_ots_keys".
-
-clone import Subtype as Three_NBytes with 
-   type T = W8.t list,
-   op P = fun l => size l = 3 * n
-   rename "T" as "three_n_bytes"
-   proof inhabited by (exists (nseq (3*n) W8.zero);smt(size_nseq ge0_n))
-   proof *.
 
 (* treeheight . n *)
-clone import Subtype as AuthPath with
+clone export Subtype as AuthPath with
   type T = nbytes list,
   op P = fun l => size l = d
   rename "T" as "auth_path"
-  proof inhabited by admit
+  proof inhabited by (exists (mkseq (fun i => witness) d);rewrite /P size_mkseq;smt(ge0_d))
   proof *.
 
 (******************************************************************************)
